{
 "cells": [
  {
   "cell_type": "code",
   "execution_count": 1,
   "id": "f6a37927-851a-41c2-bb5e-7a8752abe7b8",
   "metadata": {},
   "outputs": [],
   "source": [
    "import ollama"
   ]
  },
  {
   "cell_type": "code",
   "execution_count": 4,
   "id": "55f5db4e-6695-493c-b9c5-ffa585bb1d1c",
   "metadata": {},
   "outputs": [],
   "source": [
    "response = ollama.chat(model='deepseek-r1:7b', \n",
    "                       messages=[\n",
    "                           {\"role\": \"user\", \"content\": \"Write a python function to calculate fibonacci\"}\n",
    "                       ])"
   ]
  },
  {
   "cell_type": "code",
   "execution_count": 7,
   "id": "51d4db98-c51a-48b9-99a0-10dc23032507",
   "metadata": {},
   "outputs": [
    {
     "data": {
      "text/plain": [
       "\"<think>\\nOkay, I need to write a Python function to calculate the Fibonacci sequence. Let's see... The Fibonacci sequence starts with 0 and 1, and each subsequent number is the sum of the two preceding ones. So it goes 0, 1, 1, 2, 3, 5, 8, etc.\\n\\nHmm, so I should probably create a function that returns the nth term in the sequence. But wait, what's considered the first term? Because sometimes people define it starting at index 0 or 1. Let me think: If the function is called with n=0, it should return 0; for n=1, return 1; and so on.\\n\\nI'll start by considering how to handle different cases. Maybe I can check if n is 0 or 1 and return those values directly. For other values of n, I need a loop that builds up the sequence step by step.\\n\\nAnother approach could be using recursion. The recursive definition for Fibonacci is F(n) = F(n-1) + F(n-2), with base cases F(0)=0 and F(1)=1. But recursion might not be efficient for large n because it has an exponential time complexity, which isn't great for big numbers.\\n\\nWait, but if the function needs to handle very large n values efficiently, maybe I should use an iterative approach instead of recursion to avoid stack issues. So perhaps using a loop is better here.\\n\\nLet me outline the steps:\\n\\n1. Handle base cases where n is 0 or 1.\\n2. For larger n, iterate from 2 up to n, calculating each Fibonacci number by summing the previous two numbers.\\n3. Keep track of the current and previous values to update as we go along.\\n\\nI can initialize variables a = 0 and b = 1, which are F(0) and F(1). Then for each step from 2 to n, calculate c = a + b, then set a = b and b = c. Repeat this until I reach the desired term.\\n\\nWait, but what if someone calls the function with n less than 0? Well, Fibonacci numbers are typically defined for non-negative integers, so maybe I should add a check to ensure that n is non-negative. Otherwise, return 0 or raise an error.\\n\\nPutting it all together: The function will first handle edge cases where n is 0 or 1, then use a loop starting from 2 up to n-1 (since the list starts at 0) and calculate each term by adding the two previous terms.\\n\\nLet me sketch this out:\\n\\ndef fibonacci(n):\\n    if n <= 0:\\n        return 0\\n    elif n == 1 or n == 2:\\n        return 1\\n    else:\\n        a, b = 0, 1\\n        for i in range(3, n+1):\\n            c = a + b\\n            a = b\\n            b = c\\n        return b\\n\\nWait, but for n=3, the loop runs once. Let's test:\\n\\ni starts at 3, compute c = 0+1=1. Then a becomes 1, b becomes 1. So for i=3, returns b which is 1. That's correct as F(3)=2? Wait no, wait: Let me check the indexes again.\\n\\nWait in my code above:\\n\\nWhen n is 3, the loop runs from 3 to 3 (inclusive). Inside, c = a + b, where a was 0 and b was 1. So c=1. Then a becomes 1, b becomes 1. The function returns b, which is now 1. But F(3) should be 2.\\n\\nWait that's incorrect. What went wrong here?\\n\\nAh, because for n=3, the loop runs once (since it starts at 3 and ends at n inclusive). Wait no: in my code above, the range is from 3 to n+1? Or wait:\\n\\nNo, the function as written has a for i in range(3, n+1): which would be for 3,4,...n. Because in Python, range is exclusive on the upper end.\\n\\nWait wait no: range(3, n+1) includes up to n. So for example, if n=5, it's 3,4,5. So for each iteration i from 3 up to and including n, which makes sense because F(n) depends on F(n-1) and F(n-2), so we need all the previous terms.\\n\\nBut in my code above, when computing c as a + b, then a becomes b, and b becomes c. So for each step i:\\n\\ni=3: compute F(3)=F(2)+F(1)=1+1=2 → then a=1 (F(2)), b=2 (F(3))\\ni=4: compute F(4) = F(3) + F(2) = 2+1=3 → a becomes 2, b becomes 3\\ni=5: compute F(5)=3+2=5 → a=3, b=5\\n\\nBut when the function returns b after i reaches n.\\n\\nSo for example:\\n\\nTesting n=0: return 0.\\nn=1: return 1.\\nn=2: return 1.\\nn=3: loop runs once (i=3). c = 0+1=1. a becomes 1, b becomes 1. Then returns b which is 1? But that's incorrect because F(3) should be 2.\\n\\nWait wait no:\\n\\nHold on, the code as written:\\n\\nFor n=5, it would run i from 3 to 5 (inclusive). Let me see step by step:\\n\\ni=3: c = a(0)+b(1)=1 → a becomes 1, b becomes 1. Return b=1.\\n\\nBut F(3) is indeed 2? Wait no:\\n\\nWait the initial variables are a=0, b=1 (F(0), F(1)).\\n\\nFor i=2: c = a + b = 0+1=1 → F(2)=1. So that's correct.\\n\\nSo for i in range(3, n+1):\\n\\nAt each step:\\n\\ni=3: compute F(3) as F(2)+F(1)=1+1=2. Then a becomes F(1), b becomes 2.\\ni=4: compute F(4) = F(3)+F(2) → 2 + 1 =3. So after i=4, a is 1, b is 3.\\ni=5: compute F(5)=3+2=5.\\n\\nWait so when the loop runs up to n, it's for each step computing F(n). But in my code, inside the loop, c is computed as a + b. Then a becomes b, and b becomes c. So after each iteration:\\n\\nAt i=k: c = F(k-1) + F(k-2) → because a was F(k-3), b was F(k-4)? Wait no.\\n\\nWait wait for initial steps:\\n\\na=0 (F(0)), b=1(F(1)).\\n\\ni=2 is in the loop, which is when n >= 2. So i runs from 3 to n?\\n\\nNo, because if n is 5, and the loop starts at 3, it will run for 3,4,5.\\n\\nWait I'm getting a bit confused. Let me write out the steps for each n:\\n\\nLet's compute F(n) using this code for some small values of n.\\n\\nCase 1: n=0 → return 0.\\nCase 2: n=1 → return 1.\\nCase 3: n=2 → return 1.\\nCase 4: n=3:\\n- loop runs i from 3 to 3 (inclusive).\\nc = a + b → 0+1=1. Then a becomes 1, b becomes 1.\\nreturn b which is 1. But F(3) should be 2.\\n\\nWait that's an issue. So the code as written returns 1 for n=3, but it should return 2.\\n\\nAh! I see where I made a mistake. Because when i starts at 3, in the first iteration:\\n\\ni=3: c = a (0) + b (1) → 1\\nthen a becomes 1, b becomes 1.\\nSo after this iteration, F(3)=c is 1. But that's incorrect because F(3) should be 2.\\n\\nAh! So the code as written is returning F(n-1), not F(n). Because for i=3:\\n\\nWe have c = F(2) + F(1) → 1+1=2, which is correct.\\n\\nBut in my current code, the initial a and b are F(0)=0 and F(1)=1. So when we compute c as a + b, it's actually calculating F(i-2)+F(i-3). Wait no:\\n\\nWait wait: Let me think about how this loop works step by step.\\n\\nSuppose n is 5.\\n\\ni=3:\\nc = a + b → 0+1=1 → which is F(3) - but according to the Fibonacci sequence, F(3)=2. So that's wrong.\\n\\nAh! I see my mistake now. Let me re-examine the initial setup of the loop.\\n\\nIf the function for i in range(3, n+1):\\n\\nFor each iteration:\\n\\nc = a + b → which is F(i-2) + F(i-3). Because a was F(k-4), and b was F(k-5).\\n\\nWait no, let's see:\\n\\nAfter initializing a=0, b=1 (F(0)=0, F(1)=1).\\n\\nFor i=3:\\n\\nc = 0 +1=1 → which is F(2) ?\\n\\nNo. Because for i=3, the step would be c = F(i-2 -1) + F(i-3 -1). Not sure.\\n\\nWait maybe it's better to write down each step with n and see what happens.\\n\\nn=5:\\n\\nLoop runs for i from 3 to 5 (inclusive), so three iterations: i=3,4,5.\\n\\nLet me track a and b after each iteration:\\n\\nInitially:\\na = F(0) =0\\nb = F(1)=1\\n\\ni=3:\\nc = a + b → 0+1=1. So c is F(2). Because F(2) =1.\\nThen, set a = b (which was 1), and b = c (which is now 1). So after this iteration, a=F(1)=1, b=F(3)=1.\\n\\ni=4:\\nc =a +b → 1+1=2. Which should be F(3)=2.\\nSet a =b (now 1), b=c (now 2).\\nSo now a=F(2)=1, b=F(4)=2.\\n\\ni=5:\\nc=a + b →1 +2=3. So c is 3, which is F(4). Because F(4) should be 3.\\nSet a =b (2), b=c (3).\\nSo now a=F(3)=2, b=F(5)=3.\\n\\nFinally, return b=3. Which for n=5 is correct because F(5) is indeed 5?\\n\\nWait wait no! Because when i reaches 5, c is computed as F(4) + F(3). But the loop returns b after processing all iterations except possibly the last one.\\n\\nLet me retrace:\\n\\nn =5: so i runs from 3 to 5 (inclusive):\\n\\ni=3: a becomes b (1), b becomes c (1)\\nSo after i=3:\\na=F(1)=1, b=F(3)=1\\nSum is F(2).\\n\\ni=4: a is now 1 (F(1)), b is 1. So c =1+1=2 → F(3).\\nSet a=b=1, b=c=2.\\nAfter i=4:\\na=F(2)=1, b=F(4)=2\\nSum is F(3).\\n\\ni=5: a is 1 (F(2)), b is 2 (F(4)). So c =1 + 2 =3 → which is F(4).\\nSet a=b=2 (F(3)), b=c=3 (F(5)).\\nSo after this iteration, return b=3. But for n=5, the function should return F(5)=5.\\n\\nWait that's not correct because according to my previous calculation when i=5, c is 3, which would mean that the code is incorrect.\\n\\nWhat am I missing here? Oh wait, perhaps the loop runs from 2 to n-1 or something else. Or maybe the initial setup of a and b is wrong.\\n\\nWait no: Let me think about what the loop should do.\\n\\nThe correct approach for this algorithm:\\n\\nWe need to compute F(n) where F(0)=0, F(1)=1, and F(k) = F(k-1)+F(k-2).\\n\\nTo compute F(n), we can initialize two variables, a=F(0)=0, b=F(1)=1.\\n\\nThen, for each step from 2 to n:\\n\\nc =a +b → F(2)\\n\\nthen set a =b, b =c.\\n\\nThis continues until we reach the desired term.\\n\\nSo for example, when computing F(n):\\n\\nn=5: steps are as follows:\\nstep 0: a=0 (F(0)), b=1(F(1))\\nstep 1: c =a +b → F(2)=1. a becomes b (1), b becomes 1.\\nstep 2: c =1+1=2. a becomes1, b=2.\\nstep3: c=1+2=3. a becomes2, b=3.\\n\\nAfter all steps up to n, which is 5? Wait no, in this case we've done step 0 to step n-2.\\n\\nWait let me model it correctly:\\n\\nTo compute F(n), for each k from 2 to n inclusive:\\n\\nSo for k starting at 2 until k =n:\\nc = a +b\\na = b\\nb = c\\n\\nYes, that's the correct approach. So in code terms, we would loop from k=2 up to k=n.\\n\\nBut initially, a is F(0)=0, and b=F(1)=1.\\n\\nSo for each step:\\n\\ncurrent_step = 2 → compute c =a +b → which is F(2)\\nset a =b (now 1) → this is F(k-1)=F(1)\\nset b =c (now 1) → which becomes F(2)\\n\\nSimilarly, next step k=3: compute c =1+1=2=F(3), set a to previous b (which was1), and set b to c.\\n\\nSo for each iteration, we're effectively moving from the current F(k-1) and F(k-2) to F(k).\\n\\nThus, after n steps, when k reaches n, b will hold F(n).\\n\\nIn code terms:\\n\\nn = 5\\n\\nInitialize a=0, b=1\\n\\nfor k in range(2, n+1):\\n\\n    c =a +b\\n\\n    a =b\\n\\n    b =c\\n\\nAfter loop: return b.\\n\\nSo for n=5, the loop runs from 2 to 5 inclusive: steps k=2,3,4,5. Let's see:\\n\\nk=2:\\nc=0+1=1 → F(2)\\na becomes 1 (F(1))\\nb becomes1 (F(2))\\n\\nk=3:\\nc=1+1=2 → F(3)\\na becomes1\\nb becomes2\\n\\nk=4:\\nc=1+2=3→ F(4)\\na becomes2\\nb becomes3\\n\\nk=5:\\nc=2+3=5→ F(5)\\na becomes3\\nb becomes5.\\n\\nSo after the loop, b is 5. Which is correct.\\n\\nIn my earlier case for n=5, I messed up the steps because in the initial code's example, when i ran from 3 to 5, perhaps that was incorrect.\\n\\nBut according to this approach, with k starting at 2, it works correctly.\\n\\nSo the error earlier was thinking of looping from 3 to 5. But actually, for n=5, you need to loop from 2 to 5 inclusive, so steps 4 times (from 2 to5 is 4 numbers: 2,3,4,5). Let me count:\\n\\nn=5 → k runs as 2,3,4,5. So four iterations.\\n\\nIn each iteration, we compute c and update a and b.\\n\\nSo in code terms, for the problem of calculating F(n):\\n\\nWe need to write a loop from k=2 up to n (inclusive) steps, each time computing c =a +b, then setting a to previous b, and b to c. So after all iterations, b will be the desired value.\\n\\nIn Python, this can be written as:\\n\\ndef compute_F(n):\\n    if n ==0:\\n        return 0\\n    elif n ==1:\\n        return 1\\n    a, b = 0,1\\n    for k in range(2, n+1):  # since k is from 2 to n inclusive.\\n        c =a +b\\n        a = b\\n        b =c\\n    return b\\n\\nWait let's test this function.\\n\\nn=0 → returns 0. Correct.\\nn=1 → returns 1. Correct.\\nn=2: loop runs once (k=2). Compute c=0+1=1, then a=1, b=1. So function returns 1. Which is correct because F(2)=1.\\n\\nn=3:\\n\\nLoop runs k=2 and 3:\\nAfter k=2: a=1, b=1.\\nk=3: compute c=1+1=2 → a becomes1, b becomes2. return 2.\\n\\nWhich is correct as F(3) =2.\\n\\nn=5: returns 5, which we saw earlier.\\n\\nSo in the initial problem statement, when n was 5, it would return 5, but according to my previous mistake, I thought that after loop k=5, b was 3. But no, because with this code, the function will correctly compute F(5) as 5.\\n\\nBut wait earlier I had a miscalculation in another example where n=4:\\n\\nn=4: after each step:\\n\\nk=2 → c=1, a=1, b=1.\\nk=3 → c=2, a=1→b becomes2.\\nk=4 → c=3, a becomes 2 (from previous step's b), b becomes3.\\n\\nSo function returns3. Correct as F(4)=3.\\n\\nHmm, but in my earlier test case where n=5, I had an error because of incorrect loop steps.\\n\\nNow the code seems correct.\\n\\nBut perhaps we can make it more efficient or optimize for better performance.\\n\\nWait, given that this is a straightforward implementation, perhaps even though O(n) time and space. But for coding challenges, sometimes they prefer to handle larger n with better space, but in Python, using variables would be manageable.\\n\\nAlternatively, for very large n (like 10^6 or more), an iterative approach may not be the most efficient because of function call overhead per step. So perhaps we can implement it as a loop that increments variables instead.\\n\\nBut in this problem statement, I don't see any constraints on the size of n—though in Python, even for very large n (like 1e6), it should handle the computation within acceptable time.\\n\\nSo perhaps implementing the code with a function is fine. So let's write the function as above.\\n\\nTesting:\\n\\nCase 1: n=0 → returns 0.\\nCase 2: n=5 → returns5.\\nCase3:n=2→returns1.\\nCase4:n=3→returns2.\\nAll are correct.\\n\\nAnother case, what about n=6?\\n\\nCompute F(6): should be5.\\n\\nWait, let me compute it step by step:\\n\\nn=0 → return 0\\nn=1 →return1\\nn=2: returns1 (as per code)\\nWait wait. Wait no—earlier I thought the function for n=2 returns1 correctly? But according to this manual computation earlier.\\n\\nWait in the initial test, when k runs from2 ton inclusive, after each step:\\n\\nFor n=2, loop only runs once (k=2).\\n\\na and b are 0 and1.\\n\\nc =0+1=1. a becomes1, b becomes1.\\n\\nSo returns1. Correct as F(2)=1.\\n\\nn=3: after k=2,3 → returns2.\\n\\nWhich is correct as F(3)=2.\\n\\nSo for n=4: loop runs 2,3,4:\\n\\nAfter step k=4, a was set to previous b's value, which was 2 (from step k=3 where a was1 and b became2).\\n\\nc =1 +2=3 → a becomes2, b becomes3.\\n\\nThus function returns3. Correct as F(4)=3.\\n\\nn=5: loops from2 to5: returns5. Correct.\\n\\nn=6:\\n\\nAfter each iteration:\\n\\nk runs 2-6: steps 5.\\n\\nLet's see step by step:\\n\\nInitial a=0,b=1.\\n\\nStep k=2: c=1, a becomes1, b becomes1.\\nstep k=3: c =1+1=2 →a=1 (previous b), b=2.\\nstep k=4: c =1 +2=3→ a=2, b=3.\\nstep k=5: c=2+3=5→ a=3, b=5.\\nstep k=6: c=3+5=8→a=5, b=8.\\n\\nSo function returns 8. Which is correct as F(6)=8.\\n\\nSo yes, the code seems to handle it correctly.\\n\\nHence, implementing this function should solve the problem.\\n\\nNow, what about n being 0 or1?\\n\\nYes:\\n\\nn=0: return0.\\nn=1: return1.\\n\\nThus, the function will cover all possible cases.\\n\\nTherefore, the Python solution is as follows.\\n\\nBut in code, perhaps using a loop variable and variables to track F(k-2), F(k-1), and current.\\n\\nAlternatively, since we can optimize for space—since only keeping two variables (a and b)—we don't need a list or anything. So no extra memory required beyond the function's variables, which is better in terms of code efficiency, especially if n is large.\\n\\nSo now, coding this function.\\n</think>\\n\\nTo solve this problem, we need to compute the nth Fibonacci number efficiently. The Fibonacci sequence is defined such that each number is the sum of the two preceding ones, starting from 0 and 1. We will use an iterative approach to achieve this efficiently.\\n\\n### Approach\\nThe approach involves iterating through the sequence while maintaining only the last two numbers at any given step. This method ensures that we do not use extra space proportional to n, making it more efficient in terms of both time and space complexity.\\n\\nHere's a detailed breakdown of the steps:\\n1. **Initialization**: Start with the first two Fibonacci numbers, 0 and 1.\\n2. **Iteration**: For each number from 2 up to n (inclusive), compute the next Fibonacci number as the sum of the previous two numbers.\\n3. **Update Variables**: After computing each new Fibonacci number, update the variables to the last two computed numbers for the next iteration.\\n\\nThis approach ensures that we only use constant space (O(1)) and linear time complexity (O(n)), making it very efficient even for large values of n.\\n\\n### Solution Code\\n```python\\ndef fibonacci(n):\\n    if n == 0:\\n        return 0\\n    elif n == 1:\\n        return 1\\n    else:\\n        a, b = 0, 1\\n        for _ in range(2, n + 1):\\n            c = a + b\\n            a, b = b, c\\n        return b\\n```\\n\\n### Explanation\\nThe function `fibonacci` computes the nth Fibonacci number using an iterative approach:\\n- **Base Cases**: If n is 0, it returns 0. If n is 1, it returns 1.\\n- **Iteration Loop**: For values of n greater than 1, we initialize two variables `a` and `b` to 0 and 1, respectively. These represent the first two Fibonacci numbers.\\n- **Loop Execution**: We iterate from 2 up to n (inclusive). In each iteration, we compute the next Fibonacci number as the sum of `a` and `b`, then update `a` and `b` to the last two computed values.\\n- **Return Result**: After completing the loop, `b` holds the nth Fibonacci number, which is then returned.\\n\\nThis method efficiently computes the Fibonacci number in linear time with constant space complexity, making it suitable for large inputs.\""
      ]
     },
     "execution_count": 7,
     "metadata": {},
     "output_type": "execute_result"
    }
   ],
   "source": [
    "response['message']['content']"
   ]
  },
  {
   "cell_type": "code",
   "execution_count": null,
   "id": "27d7f89a-7934-4cb0-86ff-db27b3d1e7a9",
   "metadata": {},
   "outputs": [],
   "source": []
  }
 ],
 "metadata": {
  "kernelspec": {
   "display_name": "Python 3 (ipykernel)",
   "language": "python",
   "name": "python3"
  },
  "language_info": {
   "codemirror_mode": {
    "name": "ipython",
    "version": 3
   },
   "file_extension": ".py",
   "mimetype": "text/x-python",
   "name": "python",
   "nbconvert_exporter": "python",
   "pygments_lexer": "ipython3",
   "version": "3.11.9"
  }
 },
 "nbformat": 4,
 "nbformat_minor": 5
}
